---
title: "B-spline notes"
author: "Serguei Sokol"
date: "13/04/2022"
output: html_document
editor_options: 
  markdown: 
    wrap: 72
---

```{r setup, include=FALSE}
knitr::opts_chunk$set(echo = TRUE)
```

## B-spline recursive definition

Cox-de Boor formula:

$$
B_{i,0} := \left\{
\begin{array}{ll}
  1\ \ \text{if}\ t_i \leq x \lt t_{i+1} \\
  0\ \ \text{otherwise.}
\end{array}
\right.
$$
$$ B_{i,k} := \frac{x-t_i}{t_{i+k} - t_i} B_{i,k-1}(x) + \frac{t_{i+k+1} - x}{t_{i+k+1} - t_{i+1}} B_{i+1,k-1}(x) $$

## First derivative

$$ \frac{dB_{i,k}(x)}{dx} = k \left( \frac{B_{i,k-1}(x)}{t_{i+k} - t_i} - \frac{B_{i+1,k-1}(x)}{t_{i+k+1} - t_{i+1}}  \right) $$

This implies that

$$ \frac{d}{dx}\sum_{i} \alpha_i B_{i,k} =  \sum_{i=r-k+2}^{s-1} k \frac{\alpha_i - \alpha_{i-1}}{t_{i+k} - t_i} B_{i,k-1} \ \ \text{on}\ \ [t_r, t_s] $$

## Integral

Let $$ \beta_i = k \frac{\alpha_i - \alpha_{i-1}}{t_{i+k} - t_i} $$ Then
$$ \int_0^\zeta  \frac{d}{dx}\sum_{i} \alpha_i B_{i,k} \ dx =  \int_0^\zeta \sum_{i=r-k+2}^{s-1} \beta_i B_{i,k-1} \ dx $$
$$ \sum_{i} \alpha_i B_{i,k} \mid_0^\zeta = \int_0^\zeta \sum_{i=r-k+2}^{s-1} \beta_i B_{i,k-1} \ dx $$
If $\beta_i$ is considered as known and we have to find $\alpha_i$, we
get $$
 \alpha_i = \beta_i \frac{t_{i+k}-t_i}{k} + \alpha_{i-1}
$$ here $\alpha_0$ being a freely defined constant. In term of
cumulative sum, it gives $$
 \alpha_j = \sum_{i=0}^j \beta_i \frac{t_{i+k}-t_i}{k}
$$
